Q1 working version. needs more refinement

MergeSort.dfy
@@ -11,13 +11,216 @@ predicate SortedSequence(q: seq<int>)
 
 method MergeSort(a: array<int>) returns (b: array<int>)
 	ensures b.Length == a.Length && Sorted(b) && multiset(a[..]) == multiset(b[..])
-	decreases a.Length
+	decreases a.Length, 1
+	{
+		if a.Length <= 1
+		{
+			b := a;
+		}
+		else
+		{
+			b := Merge_NotEmptyOrSingle(a);
+		}
+	}
+
+method Merge_NotEmptyOrSingle(a: array<int>) returns (b: array<int>)
+// todo: refine
+	requires a.Length > 1
+	ensures b.Length == a.Length && Sorted(b) && multiset(a[..]) == multiset(b[..])
+	decreases a.Length, 0
+{
+	var mid := a.Length / 2;
+	var left, right := a[.. mid], a[mid..];
+
+	assert(a[..] == left[..] + right[..]);
+
+	var leftArr := SeqToArray(left);
+	var rightArr := SeqToArray(right);
+
+	assert(leftArr.Length < a.Length && rightArr.Length < a.Length);
+	
+	leftArr := MergeSort(leftArr);
+	rightArr := MergeSort(rightArr);
+
+	b := new int[a.Length];
+	Merge(b, leftArr, rightArr);
+}
+
+method SeqToArray(a: seq<int>) returns (b: array<int>)
+ensures a == b[..]
+{
+	b := new int[|a|];
+	var i := 0;
+
+	while i < |a|
+	decreases |a| - i
+	invariant |a| >= i
+	invariant a[..i] == b[..i]
+	{
+		b[i] := a[i];
+		i := i + 1;
+	}
+}
+
 
 method Merge(b: array<int>, c: array<int>, d: array<int>)
 	requires b != c && b != d && b.Length == c.Length + d.Length
 	requires Sorted(c) && Sorted(d)
 	ensures Sorted(b) && multiset(b[..]) == multiset(c[..])+multiset(d[..])
 	modifies b
+	{
+		assert(MergeIterationInvariant(b, c, d, 0, 0));
+		Iterate(b, c, d, 0, 0);
+	}
+
+predicate MergeIterationInvariant(b: array<int>, c: array<int>, d: array<int>, i : nat, j:nat)
+	reads(b)
+	reads(c)
+	reads(d)
+{	
+	b != c && b != d && b.Length == c.Length + d.Length
+	&& 0 <= i <= c.Length
+	&& 0 <= j <= d.Length 
+	&& i + j <= b.Length
+	&& Sorted(c)
+	&& Sorted(d)
+
+	// the current item at c, d is greater than every item in b
+	&& (i < c.Length ==> forall x :: 0 <= x < i + j ==> b[x] <= c[i])
+	&& (j < d.Length ==> forall x :: 0 <= x < i + j ==> b[x] <= d[j])
+	
+	// SortedSequence(b[..i+j]) could not be safely inlined
+	&& (forall x :: x == i+j ==> SortedSequence(b[..x]))
+
+	&& multiset(b[..i+j]) == multiset(c[..i])+multiset(d[..j])
+}
+
+method {:verify false} Iterate(b: array<int>, c: array<int>, d: array<int>, i0 : nat, j0:nat)
+	requires MergeIterationInvariant(b, c, d, i0, j0)
+	modifies b
+	ensures Sorted(b) && multiset(b[..]) == multiset(c[..])+multiset(d[..])
+
+	{
+		var i, j := i0, j0;
+
+		while i+j < b.Length
+			invariant MergeIterationInvariant(b, c, d, i, j);
+			decreases b.Length - (i+j)
+			{
+				i, j := MergeIterateStep(b, c, d, i, j);
+			}
+
+	// lemma that proves that inv + !guard => post		
+	}
+
+
+method MergeIterateStep(b: array<int>, c: array<int>, d: array<int>, i0 : nat, j0:nat) returns (i:nat, j:nat)
+	requires b.Length > i0 + j0
+	requires MergeIterationInvariant(b, c, d, i0, j0)
+	ensures MergeIterationInvariant(b, c, d, i, j)
+	
+	modifies b
+
+{
+	// todo: seperate to a weaken precondition function?
+	MergeLoopLemma(b, c, d, i0, j0);
+
+	if i0 == c.Length
+	{
+		// Weaken precondition to match TakeFrom's pre
+		i, j := TakeFromD(b, c, d, i0, j0);
+	}
+	else if j0 == d.Length
+	{
+		// Weaken precondition to match TakeFrom's pre
+		i, j := TakeFromC(b, c, d, i0, j0);
+	}
+	else if c[i0] > d[j0]
+	{
+		// Weaken precondition to match TakeFrom's pre
+		i, j := TakeFromD(b, c, d, i0, j0);
+	}
+	else
+	{
+		// Weaken precondition to match TakeFrom's pre
+		i, j := TakeFromC(b, c, d, i0, j0);
+	}
+}
+
+
+
+method TakeFromC(b: array<int>, c: array<int>, d: array<int>, i0 : nat, j0:nat) returns (i:nat, j:nat)
+	requires MergeIterationInvariant(b, c, d, i0, j0)
+	requires i0 < c.Length
+	requires j0 == d.Length || d[j0] >= c[i0]
+	ensures MergeIterationInvariant(b, c, d, i, j)
+
+	modifies b
+	{
+		assert(MergeIterationInvariant(b, c, d, i0, j0));
+
+		// TODO: prove
+		b[i0 + j0] := c[i0];
+
+		assert(MergeIterationInvariant(b, c, d, i0, j0));
+
+		TakeFromCLemma(b, c, d, i0, j0);
+		i, j := i0 + 1, j0;
+	}
+
+method TakeFromD(b: array<int>, c: array<int>, d: array<int>, i0 : nat, j0:nat) returns (i:nat, j:nat)
+	requires MergeIterationInvariant(b, c, d, i0, j0)
+	requires j0 < d.Length
+	requires i0 == c.Length || c[i0] >= d[j0]
+	ensures MergeIterationInvariant(b, c, d, i, j)
+
+	modifies b
+	{	
+		assert(MergeIterationInvariant(b, c, d, i0, j0));
+		ghost var k := i0+j0;
+
+		// TODO: prove
+		b[i0 + j0] := d[j0];
+		
+		TakeFromDLemma(b, c, d, i0, j0);
+		i, j := i0, j0 + 1;
+	}	
+
+lemma TakeFromCLemma(b: array<int>, c: array<int>, d: array<int>, i0 : nat, j0:nat)
+	requires MergeIterationInvariant(b, c, d, i0, j0)
+	requires i0 < c.Length
+	requires j0 == d.Length || d[j0] >= c[i0]
+	requires b[i0 + j0] == c[i0]
+	ensures MergeIterationInvariant(b, c, d, i0+1, j0)
+	{
+		ghost var i, j := i0 + 1, j0;
+		ghost var k := i + j;
+
+		assert(SortedSequence(b[..k]));
+	}
+
+lemma TakeFromDLemma(b: array<int>, c: array<int>, d: array<int>, i0 : nat, j0:nat)
+	requires MergeIterationInvariant(b, c, d, i0, j0)
+	requires j0 < d.Length
+	requires i0 == c.Length || c[i0] >= d[j0]
+	requires b[i0 + j0] == d[j0]
+	ensures MergeIterationInvariant(b, c, d, i0, j0+1)
+	{
+
+		ghost var i, j := i0, j0 + 1;
+		ghost var k := i + j;
+		assert(SortedSequence(b[..k]));
+	}
+
+
+
+lemma MergeLoopLemma(b: array<int>, c: array<int>, d: array<int>, i : nat, j:nat)
+requires MergeIterationInvariant(b, c, d, i, j)
+requires i+j < b.Length
+ensures i == c.Length ==> j < d.Length
+ensures j == d.Length ==> i < c.Length
+{
+}
 
 method Main() {
 	var a := new int[3];
@@ -31,3 +234,5 @@ method Main() {
 	assert Sorted(a);
 	assert a[..] == [4,6,8];
 }
+
+
